theories/pure_complete/samples_one.v
@@ -1,0 +1,322 @@
+From stdpp Require Import prelude coPset namespaces.
+From iris.proofmode Require Import proofmode.
+From iris.algebra Require Import list.
+From clutch.common Require Import language ectx_language ectxi_language locations.
+From clutch.prelude Require Import fin.
+From clutch.prob_lang Require Import notation lang.
+From clutch.prob_lang.spec Require Import spec_ra spec_rules spec_tactics.
+From clutch.approxis Require Import ectx_lifting app_weakestpre model.
+From clutch.approxis Require Export proofmode primitive_laws coupling_rules.
+From clutch.base_logic Require Export spec_update.
+From clutch.pure_complete Require Import pure tachis_ert prob_additional.
+From Coq.Logic Require Import ClassicalEpsilon.
+Local Open Scope R.
+
+Inductive SamplesOneTape : loc -> expr -> Prop :=
+  | SamplesOneTapeRand t e2 (H1 : SamplesOneTape t e2) :
+    SamplesOneTape t (Rand e2 (Val (LitV (LitLoc t))))
+  | SamplesOneTapeIf t e2 e3 e4 (H1 : SamplesOneTape t e2) (H2 : SamplesOneTape t e3) (H3 : SamplesOneTape t e4) :
+    SamplesOneTape t (if: e2 then e3 else e4)%E
+  | SamplesOneTapeVar t s : 
+    SamplesOneTape t (Var s)
+  | SamplesOneTapePair t e2 e3 (H : SamplesOneTape t e2) (H1 : SamplesOneTape t e3) :
+    SamplesOneTape t (Pair e2 e3)
+  | SamplesOneTapeFst t e2 (H : SamplesOneTape t e2) :
+    SamplesOneTape t (Fst e2)
+  | SamplesOneTapeSnd t e2 (H : SamplesOneTape t e2) :
+    SamplesOneTape t (Snd e2)
+  | SamplesOneTapeInjL t e2 (H : SamplesOneTape t e2) :
+    SamplesOneTape t (InjL e2)
+  | SamplesOneTapeInjR t e2 (H : SamplesOneTape t e2) :
+    SamplesOneTape t (InjR e2)
+  | SamplesOneTapeCase t e2 e3 e4 (H : SamplesOneTape t e2) (H1 : SamplesOneTape t e3) (H2 : SamplesOneTape t e4) :
+    SamplesOneTape t (Case e2 e3 e4)
+  | SamplesOneTapeRec f x t e2 (H : SamplesOneTape t e2) :
+    SamplesOneTape t (Rec f x e2)
+  | SamplesOneTapeApp t e2 e3 (H : SamplesOneTape t e2) (H1 : SamplesOneTape t e3) :
+    SamplesOneTape t (App e2 e3)
+  | SamplesOneTapeTick t e2 (H : SamplesOneTape t e2) :
+    SamplesOneTape t (Tick e2)
+  | SamplesOneTapeUnOp t e2 (H : SamplesOneTape t e2) (op : un_op) :
+    SamplesOneTape t (UnOp op e2)
+  | SamplesOneTapeBinOp t e2 e3 (H : SamplesOneTape t e2) (H1 : SamplesOneTape t e3) (op : bin_op) :
+    SamplesOneTape t (BinOp op e2 e3)
+  | SamplesOneTapeVal t v (H : SamplesOneTapeV t v) :
+    SamplesOneTape t (Val v)
+with SamplesOneTapeV : loc -> val -> Prop :=
+  | SamplesOneTapeVRecV f x t e2 (H : SamplesOneTape t e2) :
+    SamplesOneTapeV t (RecV f x e2)
+  | SamplesOneTapeVPairV v1 v2 t (H : SamplesOneTapeV t v1) (H1 : SamplesOneTapeV t v2) :
+    SamplesOneTapeV t (PairV v1 v2)
+  | SamplesOneTapeVInjLV v t (H : SamplesOneTapeV t v) :
+    SamplesOneTapeV t (InjLV v)
+  | SamplesOneTapeVInjRV v t (H : SamplesOneTapeV t v) :
+    SamplesOneTapeV t (InjRV v)
+  | SamplesOneTapeVLitV v t :
+    SamplesOneTapeV t (LitV v)
+.
+
+Inductive SamplesOneTapeItem (t : loc) : ectx_item -> Prop :=
+  | SamplesOneTapeItemAppLCtx v : SamplesOneTapeV t v -> SamplesOneTapeItem t (AppLCtx  v)
+  | SamplesOneTapeItemAppRCtx e : SamplesOneTape t e -> SamplesOneTapeItem t (AppRCtx  e)
+  | SamplesOneTapeItemUnOpCtx op : SamplesOneTapeItem t (UnOpCtx  op)
+  | SamplesOneTapeItemBinOpLCtx op v : SamplesOneTapeV t v -> SamplesOneTapeItem t (BinOpLCtx op v)
+  | SamplesOneTapeItemBinOpRCtx op e : SamplesOneTape t e -> SamplesOneTapeItem t (BinOpRCtx op e)
+  | SamplesOneTapeItemIfCtx e1 e2 : SamplesOneTape t e1 -> SamplesOneTape t e2 -> SamplesOneTapeItem t (IfCtx e1 e2)
+  | SamplesOneTapeItemPairLCtx v : SamplesOneTapeV t v -> SamplesOneTapeItem t (PairLCtx v)
+  | SamplesOneTapeItemPairRCtx e : SamplesOneTape t e -> SamplesOneTapeItem t (PairRCtx e)
+  | SamplesOneTapeItemFstCtx : SamplesOneTapeItem t FstCtx
+  | SamplesOneTapeItemSndCtx : SamplesOneTapeItem t SndCtx
+  | SamplesOneTapeItemInjLCtx : SamplesOneTapeItem t InjLCtx
+  | SamplesOneTapeItemInjRCtx : SamplesOneTapeItem t InjRCtx
+  | SamplesOneTapeItemCaseCtx e1 e2 : SamplesOneTape t e1 -> SamplesOneTape t e2 -> SamplesOneTapeItem t (CaseCtx e1 e2)
+  | SamplesOneTapeItemRandLCtx : SamplesOneTapeItem t (RandLCtx #t)
+  | SamplesOneTapeItemTickCtx : SamplesOneTapeItem t TickCtx.
+
+Lemma SamplesOneTape_fill_item Ki e l :
+  SamplesOneTape l e ->
+  SamplesOneTapeItem l Ki ->
+  SamplesOneTape l (fill_item Ki e).
+Proof.
+  intros.
+  inversion H0; simpl; 
+  econstructor; auto;
+  econstructor; auto.
+Qed.
+
+Lemma SamplesOneTape_fill K e l :
+  SamplesOneTape l e ->
+  Forall (SamplesOneTapeItem l) K ->
+  SamplesOneTape l (fill K e).
+Proof.
+  intros. 
+  revert e H.
+  induction K; auto. 
+  intros. simpl.
+  inversion H0; subst.
+  apply IHK; auto.
+  by apply SamplesOneTape_fill_item. 
+Qed.
+
+Lemma SamplesOneTape_head l e ei e' : 
+  SamplesOneTape l e ->
+  decomp_item e = Some (ei, e') ->
+  SamplesOneTape l e'.
+Proof.
+  intros.
+  inversion H; subst; simpl in *; inversion H0;
+  try (destruct e2; inversion H3; done);
+  try (destruct e3; destruct e2; inversion H4; done);
+  (destruct e2; inversion H5; done). 
+Qed.
+
+Lemma SamplesOneTape_ectx e l :
+  SamplesOneTape l e ->
+  Forall (SamplesOneTapeItem l)(decomp e).1.
+Proof.
+  simpl.
+  destruct (decomp e) eqn : Hde.
+  remember (length l0).
+  revert e e0 l0 Hde Heqn.
+  induction n.
+  {
+    intros.
+    destruct l0; inversion Heqn.
+    apply decomp_inv_nil in Hde as [Hd Hde].
+    by subst e.
+  }
+  intros.
+  rewrite decomp_unfold in Hde.
+  destruct (ectxi_language.decomp_item e) eqn : Hde'; intros.
+  2: {inversion Hde. by subst e. }
+  destruct p.
+  destruct (decomp e2) eqn: Hde2.
+  inversion Hde. subst.
+  apply Forall_app_2. 
+  {
+    eapply IHn.
+    - apply Hde2.
+    - rewrite app_length Nat.add_1_r in Heqn. by inversion Heqn.
+    - simpl in *.
+      eapply SamplesOneTape_head; eauto.
+  }
+  apply Forall_singleton. 
+  simpl in *.
+  rewrite /decomp_item in Hde'.
+  inversion H; subst; simpl in *;
+  try by inversion Hde';
+  try (destruct e3; inversion Hde'; econstructor; done);
+  try (destruct e4; destruct e3; inversion Hde'; econstructor; auto; by inversion H1). 
+Qed.
+  
+Lemma SamplesOneTape_decomp l e : 
+  SamplesOneTape l e ->
+  SamplesOneTape l (decomp e).2.
+Proof.
+  destruct (decomp e) eqn : Hde.
+  simpl.
+  remember (length l0).
+  revert e l0 e0 Hde Heqn.
+  induction n.
+  {
+    intros.
+    destruct l0; simpl in *; try by inversion Heqn.
+    apply decomp_inv_nil in Hde as [Hd Hde].
+    by subst.
+  }
+  intros.
+  rewrite decomp_unfold in Hde.
+  destruct (ectxi_language.decomp_item e) eqn : Hde'; intros.
+  2: {inversion Hde. by subst e. }
+  destruct p.
+  destruct (decomp e2) eqn: Hde2.
+  inversion Hde. subst.
+  assert (n = length l1).
+  { 
+    rewrite app_length in Heqn. 
+    rewrite Nat.add_1_r in Heqn. auto.
+  }
+  apply (IHn _ _ _ Hde2 H0).
+  by eapply SamplesOneTape_head. 
+Qed.
+
+Lemma SamplesOneTape_decomp' l e e' Ks : 
+  SamplesOneTape l e ->
+  decomp e = (Ks, e') ->
+  SamplesOneTape l e'.
+Proof.
+  intros.
+  replace e' with (decomp e).2.
+  2 : by rewrite H0.
+  by apply SamplesOneTape_decomp.
+Qed.
+
+Lemma SamplesOneTape_head_step_det l e σ N v t e' σ':
+  SamplesOneTape l e ->
+  σ.(tapes) !! l = Some (N; v :: t) ->
+  head_step e σ (e', σ') > 0 ->
+  head_step e σ (e', σ') = 1.
+Proof.
+  intros.
+  destruct e; inv_head_step;
+  try by inversion H;
+  try by apply dret_1.
+Qed.
+
+Lemma SamplesOneTape_head_step_tape l e σ N v t e' σ':
+  SamplesOneTape l e ->
+  σ.(tapes) !! l = Some (N; v :: t) ->
+  head_step e σ (e', σ') > 0 ->
+  σ'.(tapes) = σ.(tapes) ∨ σ'.(tapes) = <[l := (N; t)]>σ.(tapes).
+Proof.
+  intros.
+  destruct e; inv_head_step; 
+  auto; inversion H. 
+Qed.
+
+Lemma SamplesOneTape_step_det l e σ N v t e' σ':
+  SamplesOneTape l e ->
+  σ.(tapes) !! l = Some (N; v :: t) ->
+  step (e, σ) (e', σ') > 0 ->
+  step (e, σ) (e', σ') = 1.
+Proof.
+  rewrite /step.
+  simpl. rewrite /prim_step.
+  intros. simpl in *. 
+  destruct (decomp e) eqn : Hde.
+  rewrite Hde.
+  rewrite Hde in H1.
+  apply dmap_pos in H1 as [(e1 & σ1) (?&?)].
+  eapply dmap_one.
+  - eapply SamplesOneTape_head_step_det; eauto.
+    eapply SamplesOneTape_decomp'; eauto.
+  - eauto.
+Qed.
+
+Lemma SamplesOneTape_step_det' l e σ N v t e' σ':
+  SamplesOneTape l e ->
+  σ.(tapes) !! l = Some (N; v :: t) ->
+  step (e, σ) (e', σ') > 0 ->
+  step (e, σ) = dret (e', σ').
+Proof.
+  intros.
+  by eapply pmf_1_eq_dret, SamplesOneTape_step_det. 
+Qed.
+
+Lemma SamplesOneTape_step_state l e σ N v t e' σ':
+  SamplesOneTape l e ->
+  σ.(tapes) !! l = Some (N; v :: t) ->
+  step (e, σ) (e', σ') > 0 ->
+  σ'.(tapes) = σ.(tapes) ∨ σ'.(tapes) = <[l := (N; t)]>σ.(tapes).
+Proof.
+  rewrite /step.
+  simpl. rewrite /prim_step.
+  intros. simpl in *. 
+  destruct (decomp e) eqn : Hde.
+  rewrite Hde in H1.
+  apply dmap_pos in H1 as [(e1 & σ1) (?&?)].
+  inversion H1; subst.
+  eapply SamplesOneTape_head_step_tape.
+  - eapply SamplesOneTape_decomp'; eauto.
+  - eauto.
+  - eauto.
+Qed.
+
+Lemma SamplesOneTape_subst l x v e : 
+  SamplesOneTape l e ->
+  SamplesOneTapeV l v ->
+  SamplesOneTape l (subst x v e).
+Proof.
+  intros.
+  induction e; simpl; auto;
+  try (inversion H; subst; case_decide; auto; econstructor; by eauto); 
+  try (inversion H; subst; econstructor; by eauto).  
+Qed.
+
+Lemma SamplesOneTape_head_inv l e σ e' σ':
+  SamplesOneTape l e ->
+  head_step e σ (e', σ') > 0 ->
+  SamplesOneTape l e'.
+Proof.
+  intros.
+  inversion H; inv_head_step;
+  auto;
+  try (inversion H1; inversion H5; subst; econstructor; eauto; econstructor; done);
+  try (do 2 econstructor; done); 
+  try (econstructor; econstructor; inversion H1; inversion H2; subst; done);
+  try (inversion H1; inversion H3; subst; econstructor; done). 
+  - inversion H1. inversion H4. inversion H2. subst. 
+    destruct x, f; simpl; auto; 
+    apply SamplesOneTape_subst; auto;
+    apply SamplesOneTape_subst; auto.
+  - destruct op; destruct v; inversion H3;
+    destruct l0; inversion H3; do 2 econstructor. 
+  - destruct op, v; inversion H5; 
+    try (destruct l0; inversion H5; destruct v0; inversion H5;
+    destruct l0; inversion H5; econstructor; try econstructor;
+    destruct l1; inversion H5; by econstructor);
+    try (unfold bin_op_eval in *;
+    case_decide; try contradiction; case_decide; inversion H5;
+    subst; do 2 econstructor). 
+Qed.
+
+Lemma SamplesOneTape_inv l e σ e' σ':
+  SamplesOneTape l e ->
+  step (e, σ) (e', σ') > 0 ->
+  SamplesOneTape l e'.
+Proof.
+  unfold step.
+  simpl. unfold prim_step.
+  intros. 
+  destruct (decomp e) eqn : Hde.
+  simpl in *.
+  rewrite Hde dmap_pos in H0.
+  destruct H0 as [[e1 σ1] [Hfl Hs]].
+  inversion Hfl.
+  apply SamplesOneTape_fill.
+  - eapply SamplesOneTape_head_inv.
+    + eapply (SamplesOneTape_decomp'); last first; eauto.  
+    + eauto.
+  - replace l0 with (decomp e).1; try by rewrite Hde. 
+    by apply SamplesOneTape_ectx. 
+Qed.
